theories/enum.v
@@ -1,0 +1,294 @@
+From HB Require Import structures.
+From mathcomp Require Import all_ssreflect zify.
+From deriving Require Import deriving. 
+Require Import Program. 
+From Equations Require Import Equations.
+Require Export Containment.regex.
+From Containment Require Import tactics utils.
+
+
+Set Implicit Arguments.
+Set Maximal Implicit Insertion.
+
+Let inE := utils.inE.
+
+
+Fixpoint enum (A : Type) (n : nat) (R : seq A) := 
+match n with 
+| 0 => nil::nil 
+| n'.+1 => (compose R (enum n' R) cons)++(enum n' R)
+end.
+
+
+Lemma in_enum_nil : forall (A : eqType) n (R : seq A), nil \in enum n R. 
+Proof.
+move=> A'.
+elim;ssa.
+rewrite mem_cat H. lia.
+Qed.
+
+
+Lemma in_enum : forall (A : eqType) n R (l : seq A), size l <= n -> (forall x, x \in l -> x \in R) -> l \in enum n R. 
+Proof.
+move=> A'.
+elim;ssa. destruct l;ssa.
+destruct l. rewrite mem_cat in_enum_nil. lia.
+rewrite mem_cat. apply/orP. left.
+apply/mem_compose. eauto. eauto.
+Qed.
+
+Lemma uniq_size : forall (A : eqType) (l : seq A) R, uniq l -> (forall x, x \in l -> x \in R) -> size l <= size R.
+Proof.
+move=> A'.
+elim;ssa. 
+have : forall x, x \in l -> x \in R. eauto.
+move=> Hin. 
+move: (H _ H3 Hin). move=>Hsize.
+move: (H1 a). rewrite !inE /=. move/(_ is_true_true)=>Hr.
+apply:size_strict_sub. done. done. eauto. done.
+Qed.
+
+Lemma in_enum_uniq : forall (A : eqType) R (l : seq A), uniq l -> (forall x, x \in l -> x \in R) -> l \in enum (size R) R. 
+Proof.
+intros. apply:in_enum.  apply:uniq_size. done. done. done.
+Qed.
+
+Lemma mem_compose_cons : forall (B : eqType) (aa : seq B) bb l,   l \in compose aa bb cons -> exists a b, l = cons a b /\  a \in aa /\ b \in bb.
+Proof. move => B. elim;intros. done. 
+move : H0=>/=. rewrite mem_cat. move/orP. case. move/mapP=>[] //=. intros. inversion q. subst. 
+econ. econ.  eauto.
+
+move/H. case. ssa. subst. econ. econ. eauto.
+Qed.
+
+
+Lemma enum_inR : forall (A : eqType) n R (l : seq A) x, l \in enum n R -> x \in l -> x \in R. 
+Proof.
+move=> A'.
+elim;ssa. rewrite !inE in H. norm_eqs. done.
+rewrite mem_cat in H0. de (orP H0). 
+apply mem_compose_cons in H2. ssa. subst. 
+rewrite !inE in H1. de (orP H1). norm_eqs. done.
+eauto.
+eauto.
+Qed.
+
+Section Enum.
+Variable A : finType.
+Implicit Type (r : @regex A).
+Implicit Type (pp : @pder A * @pder A).
+Fixpoint pi r := 
+match r with 
+| Eps => nil
+| Empt => nil 
+| Event _ => Eps::nil
+| Plus r0 r1 =>  (pi r0) ++ (pi r1) 
+| Seq r0 r1 => (map (fun x => x _;_ r1)(pi r0)) ++ (pi r1) 
+| Star r0 => map (fun x => x _;_ Star r0 )(pi r0)
+end.
+Definition pi2 `(r: @regex A) := r::(pi r).
+
+
+
+
+
+Ltac lo := match goal with 
+                | [H : is_true (_ || _) |- _] => destruct (orP H);norm_eqs;try solve [ssa]
+                end.
+
+
+Lemma pi_d : forall r r' a, r' \in pd a r -> r' \in pi r.
+Proof.
+elim;ssa. move: H. case_if. done. done.
+rewrite mem_cat in H1.  rewrite mem_cat. apply/orP. lo; eauto. 
+destruct (nu _) eqn:Heqn. rewrite !mem_cat in H1 *. apply/orP. lo. 
+destruct (mapP H2). subst. left. apply/map_f;  eauto. eauto.
+destruct (mapP H1). subst. rewrite mem_cat. apply/orP. left. apply/map_f. eauto.
+destruct (mapP H0). subst.  apply/map_f. eauto.
+Qed.
+Hint Resolve pi_d.
+
+Hint Resolve map_f.
+Lemma in_pi_pd : forall r0 r1 r2 a, r1 \in pi r0 -> r2 \in pd a r1 -> r2 \in pi r0.
+Proof.
+elim;ssa.
+- rewrite !inE in H. norm_eqs. ssa. 
+- rewrite !mem_cat in H1 *.  destruct (orP H1).  
+  move: (H _ _ _ H3 H2). ssa. 
+  move: (H0 _ _ _ H3 H2). ssa. 
+- rewrite !mem_cat in H1 *. 
+  destruct (orP H1). destruct (mapP H3). subst. ssa.
+  destruct (nu _) eqn:Heqn.   rewrite mem_cat in H2. destruct (orP H2).
+  destruct (mapP H5). subst. 
+  move: (H _ _ _ H4 H6). ssa. 
+  con. apply/map_f. done. eauto. 
+  destruct (mapP H2). subst. 
+  move: (H _ _ _ H4 H5). ssa.
+  left. apply/map_f. eauto.
+  move: (H0 _ _ _ H3 H2). ssa.  
+- destruct (mapP H0). subst. ssa.
+  destruct (nu _) eqn:Heqn.   rewrite mem_cat in H1. destruct (orP H1). destruct (mapP H3). subst.
+  move: (H _ _ _ H2 H4). ssa. 
+  apply/map_f. eauto.
+  destruct (mapP H3). subst. apply:map_f. eauto.
+  destruct (mapP H1). subst. ssa.
+  move: (H _ _ _ H2 H3). ssa. apply/map_f. eauto.
+Qed.
+
+Lemma in_pd_pi : forall r0 r1 r2 a, r1 \in pd a r0 -> r2 \in pi r1 -> r2 \in pi r0.
+Proof.
+elim;ssa.
+- move:H. rifliad. norm_eqs. rewrite !inE. intros. norm_eqs. ssa.
+- rewrite !mem_cat in H1 *.  destruct (orP H1).  
+  move: (H _ _ _ H3 H2). ssa. 
+  move: (H0 _ _ _ H3 H2). ssa. 
+- rewrite !mem_cat in H1 *. 
+(*  destruct (orP H1). destruct (mapP H3). subst. ssa.*)
+  destruct (nu _) eqn:Heqn.   rewrite mem_cat in H1. destruct (orP H1).
+  destruct (mapP H3). subst. ssa.
+  rewrite mem_cat in H2. de (orP H2). de (mapP H5). subst.
+  move: (H _ _ _ H4 H6). ssa. 
+  con. apply/map_f. done. eauto. 
+  move: (H0 _ _ _ H3 H2). ssa. de (mapP H1). subst. ssa.
+  rewrite mem_cat in H2. de (orP H2). de (mapP H4). subst. ssa.
+  move: (H _ _ _ H3 H5). ssa. left. apply/map_f. done.
+- destruct (mapP H0). subst. ssa.
+  rewrite mem_cat in H1. destruct (orP H1). destruct (mapP H3). subst.
+  move: (H _ _ _ H2 H4). ssa. 
+  apply/map_f. eauto.
+  destruct (mapP H3). subst. apply:map_f. eauto.
+Qed.
+
+Lemma in_pi2_pd : forall r0 r1 r2 a, r1 \in pi2 r0 -> r2 \in pd a r1 -> r2 \in pi2 r0.
+Proof.
+intros. rewrite !inE in H. lo. rewrite !inE. apply/orP. right. eauto.
+rewrite !inE. apply/orP. right. apply/in_pi_pd. eauto. eauto.
+Qed.
+
+Lemma in_pd_pi2 : forall r0 r1 r2 a, r1 \in pd a r0 -> r2 \in pi2 r1 -> r2 \in pi2 r0.
+Proof.
+intros. rewrite !inE in H0. lo. rewrite !inE. apply/orP. right. eauto.
+rewrite !inE. apply/orP. right. apply/in_pd_pi. eauto. eauto.
+Qed.
+
+Definition pi_l (l : seq regex) := undup (flatten (map pi2 l)).
+Definition enum_pi l := (enum (size (pi_l l)) (pi_l l)).
+Definition enum_pi2 l := map undup (enum_pi l). 
+
+
+
+
+
+
+Lemma in_pd_enum_aux : forall (l l' : seq regex) a, l' \in  enum_pi2 (pd_l a l) ->  l' \in enum_pi l.
+Proof.
+intros. 
+apply:in_enum_uniq. de (mapP H). subst. apply:undup_uniq.
+intros. ssa. rewrite /enum_pi2 in H.
+de (mapP H). subst.
+rewrite /pi_l. rewrite mem_undup. 
+apply/flattenP. simpl. rewrite mem_undup in H0.
+
+move: (@enum_inR _ _ _ _ _ H1 H0).
+move=>Hin. rewrite /pi_l in Hin. rewrite mem_undup in Hin.
+de (flattenP Hin). de (mapP H2). subst. 
+rewrite /pd_l in H4. rewrite mem_undup in H4. de (flattenP H4). de (mapP H5). subst.
+econ. apply/map_f. 
+2: { apply:in_pd_pi2.  apply:H6.  done. } 
+done.
+Qed.
+
+Lemma in_pd_enum : forall (l l' : seq regex) a, l' \in  enum_pi2 (pd_l a l) ->  l' \in enum_pi2 l.
+Proof.
+intros. move: (in_pd_enum_aux _ _ _ H). intros.
+de (mapP H). subst.
+apply/mapP. econ.  eauto. symmetry. rewrite undup_id //.
+apply/undup_uniq.
+Qed.
+
+Lemma enum_pi_self : forall l, uniq l ->  l \in enum_pi l.
+Proof.
+intros. apply:in_enum_uniq. done.
+intros. rewrite /pi_l. rewrite mem_undup.
+apply/flattenP. simpl. econ. 
+apply/map_f. eauto. rewrite !inE //.
+Qed.
+
+Lemma enum_pi2_self : forall l, uniq l ->  l \in enum_pi2 l.
+Proof.
+intros. apply enum_pi_self in H as H'. 
+rewrite /enum_pi2. apply/mapP. econ. eauto. 
+rewrite undup_id //.
+Qed.
+Hint Resolve enum_pi2_self.
+
+
+Definition pair_enum ee := utils.compose (enum_pi2 ee.1) (enum_pi2 ee.2) pair. 
+Definition pair_pd_l a pp := (pd_l a pp.1,pd_l a pp.2).
+
+Lemma selfee : forall pp, uniq_pair pp ->  pp \in pair_enum pp. 
+Proof. case. intros. rewrite /uniq_pair in H. ssa.
+rewrite /pair_enum /=. apply/mem_compose;eauto.
+Qed.
+Hint Resolve selfee.
+
+Lemma in_pd_pair_enum : forall l l' a, l' \in  pair_enum (pair_pd_l a l) ->  l' \in pair_enum l.
+Proof.
+intros. rewrite /pair_enum in H.  rewrite /pair_enum. destruct l'.
+apply mem_compose2 in H. destruct H. ssa.
+destruct l. ssa. 
+apply/mem_compose. 
+apply:in_pd_enum. apply:H.
+apply:in_pd_enum. apply:H0.
+Qed.
+
+
+
+Definition r_measure ( visited : seq (pder * pder)) (l : pder * pder) := 
+size (rep_rem visited (undup (pair_enum l))). 
+
+
+(*Used in session type project*)
+Hint Resolve undup_uniq.
+Lemma measure_lt : forall V l a, uniq_pair l -> l \notin V -> r_measure (l::V) (pair_pd_l a l) < r_measure V l.
+Proof.
+move=> V l a Hun Hnotin.
+intros. rewrite /r_measure. 
+simpl. 
+destruct (l \in (pair_enum (pair_pd_l a l))) eqn:Heqn.
+- apply/size_strict_sub.
+ * apply/rem_uniq/rep_rem_uniq/undup_uniq. (*uniqueness not interesting*)
+ * intros. destruct (eqVneq x l). (* enum e0 \ e::visited <= enum e \ visited *) (*x \in left -> x \in right*)
+  **  subst. rewrite -mem_rep_iff.  rewrite mem_undup. eauto. (*x = e and \e \notin visited so x \in enum e \ visited*) (*have: uniq l. de (mapP Heqn). subst. apply:undup_uniq. move=>Hun.
+      apply/pair_enum_self. done.*) done. 
+  ** apply mem_rem2 in H;eauto. (*x != e*)
+     have : x \notin V. apply/negP=>HH. eapply rep_rem_uniq2 in HH.
+
+     2: { instantiate (1:= undup (pair_enum (pair_pd_l a l))).  done. }
+     rewrite H //= in HH. move => Heqn2.
+     move : H. rewrite -!mem_rep_iff;eauto. (*x \notin V so x \in enum e0 -> x \in enum e by main lemma*)
+     rewrite  !mem_undup. intros. apply/in_pd_pair_enum. eauto.
+ * instantiate (1 := l).  apply/negP=>HH. rewrite mem_rem_uniqF in HH. done. (*e \notin enum e0 \ e::V*)
+   apply/rep_rem_uniq/undup_uniq. 
+ * rewrite -mem_rep_iff.  rewrite mem_undup. eauto.  done.
+(*apply/pair_enum_self. 
+   have: uniq l. de (mapP Heqn). subst. apply:undup_uniq=>//. done. done.*)
+- have :  l \notin rep_rem V (undup (pair_enum (pair_pd_l a l))). 
+  apply/negP=>HH. move : Heqn. move/negP=>H2. apply/H2. 
+  apply/mem_rep_iff.  apply:Hnotin. apply/rep_rem2. done.
+  2 :  eauto.  intros. rewrite mem_undup in H. done. move => HH'. 
+
+  rewrite rem_id //=. (*e \notin enum e0, suff to show enum e0 \ V < enum e \ V *)
+  apply/size_strict_sub;eauto.   
+  * apply/rep_rem_uniq. apply/undup_uniq. (*uniquenes not interesting*)
+  * intros. have : x \notin V. apply/negP=>HH. eapply rep_rem_uniq2 in HH. 
+    2: {  instantiate (1:= undup (pair_enum (pair_pd_l a l))).  done. }
+    rewrite H //= in HH. move => Heqn2. (*x \notin V*)
+    move : H. rewrite -!mem_rep_iff. rewrite  !mem_undup. intros. 
+    apply:in_pd_pair_enum. eauto. done. done.
+(*    rewrite Heqn2. (*suff to show x \in enum e0 -> x \in enum e by main lemma*)
+    done. rewrite Heqn2. done.*)
+  * rewrite -mem_rep_iff. rewrite mem_undup. eauto. done.
+Qed.
+
+End Enum.
