theories/extensional.v
@@ -1,0 +1,203 @@
+Require Import Program. 
+From Equations Require Import Equations.  
+From mathcomp Require Import all_ssreflect zify.
+Require Import Paco.paco.
+From Containment Require Import tactics utils regex enum pred.
+Set Implicit Arguments.
+Set Maximal Implicit Insertion.
+
+
+Module Extensional (M : Pred).
+Import M.
+
+Inductive exten_gen bisim : pder -> pder-> Prop :=
+ contains_con2 l0 l1 (H0: forall e, bisim (pd_l e l0) (pd_l e l1) : Prop ) (H1: Pb l0 l1 (*has nu l0 = has nu l1*)) : exten_gen bisim l0 l1.
+
+Definition Extensional l0 l1 := paco2 exten_gen bot2 l0 l1.
+Hint Unfold  Extensional : core.
+
+Lemma exten_gen_mon: monotone2 exten_gen. 
+Proof.
+unfold monotone2. intros.  constructor. inversion IN. intros.
+auto. inversion IN. auto.  
+Qed.
+Hint Resolve exten_gen_mon : paco.
+
+
+Theorem equiv_rInd : forall l l', Extensional l l' -> forall s, P s ( (\big[Plus/Empt]_(i <- l) i))  (\big[Plus/Empt]_(i <- l') i).
+Proof.
+move=> l0 l1 HC s. 
+elim: s l0 l1  HC.
+- move=> c0 c1. intros. punfold HC. case: HC. move=> ce c3 HC HC'.
+  apply Pb_P_iff. done.
+- move=> a l IH c0 c1. move=>HC.  punfold HC. case: HC. intros.
+  case: (H0 a)=>//. intros.
+(*elim.
+  move=> c2 c3 /(_ a) [] // HC _. *)
+  apply/P_derive. apply IH. done.
+Qed.
+
+Theorem Bisim_co_ind : forall l l', (forall s, P s (\big[Plus/Empt]_(i <- l) i) (\big[Plus/Empt]_(i <- l') i)) -> Extensional l l'.
+Proof.
+pcofix CIH. move=> l l'. pfold. con. 
+intros. right. apply:CIH. intros.
+apply P_derive. apply H0.
+apply/Pb_P_iff. done.
+Qed.
+
+Lemma Extensional_equiv : forall l l', Extensional l l' <->  forall s, P s (\big[Plus/Empt]_(i <- l) i) (\big[Plus/Empt]_(i <- l') i). 
+Proof.
+intros. split. apply/equiv_rInd. apply:Bisim_co_ind.
+Qed.
+
+Hint Resolve undup_uniq.
+
+Unset Implicit Arguments.
+
+(*Less effecient, fix this later*)  
+
+Implicit Type (pp : (@pder A) * (@pder A)).
+Implicit Type (visited : seq ((@pder A) * (@pder A))).
+
+Equations bisim pp visited : bool by wf (r_measure visited pp) := 
+ bisim pp visited  with (dec (pp \in visited)) => {
+  bisim _  _ (in_left) := true;
+  bisim pp visited (in_right) with (dec (uniq_pair pp)) => { 
+        bisim pp visited _ (in_left) := (Pb pp.1 pp.2) && 
+                                        (foldInAll (index_enum A) (fun e _ => bisim (pair_pd_l e (pp)) (pp::visited)));
+        bisim pp visited _ (in_right) := false }
+ }.
+Next Obligation.
+intros.
+apply/ltP. apply:measure_lt. done. rewrite e0 //. 
+Defined.
+
+(*Effecient but awkard for proofs*)
+Equations bisim2 pp visited (H : uniq_pair pp) : bool by wf (r_measure visited pp) := 
+ bisim2 pp visited H  with (dec (pp \in visited)) => {
+  bisim2 _  _ _ (in_left) := true;
+  bisim2 pp visited _ (in_right) := (Pb pp.1 pp.2) && 
+                                           (foldInAll (index_enum A) (fun e _ => bisim2 (pair_pd_l e pp) (pp::visited) _));
+ }.
+Next Obligation. 
+intros. apply/andP.
+con. simpl. rewrite /pd_l. done.  simpl. rewrite /pd_l. done.
+Defined.
+Next Obligation.
+intros. apply/ltP. apply:measure_lt. done. rewrite e0 //. 
+Defined.
+Set Implicit Arguments.
+
+Lemma bisim12 : forall pp visited (H : uniq_pair pp), bisim pp visited -> bisim2 pp visited H.
+Proof.
+intros. funelim (bisim pp visited).
+simp bisim2. simpl. rewrite Heq. simpl. done.
+simp bisim2. rewrite Heq0. simpl.
+rewrite -Heqcall in H1. ssa.
+rewrite !foldInAllP in H3 *. 
+apply/allP. intro. intros. move: (allP H3 _ H1). move/H. move/inP: H1=>H1'. move/(_ H1')=>Hall.
+apply Hall. rewrite -Heqcall in H0. done.
+Qed.
+
+Lemma bisim21 : forall pp visited (H : uniq_pair pp), bisim2 pp visited H -> bisim pp visited.
+Proof.
+intros. funelim (bisim pp visited). rewrite -Heqcall. done.
+rewrite -Heqcall. simp bisim2 in H1. rewrite Heq0 in H1. ssa.
+rewrite !foldInAllP in H3 *. 
+apply/allP. intro. intros. move: (allP H3 _ H1). move/H. move/inP: H1=>H1'. move/(_ H1')=>Hall.
+apply Hall.  clear H0.
+rewrite e1 in H. done.
+Qed.
+
+Lemma bisim_iff : forall pp visited (H : uniq_pair pp), bisim pp visited <-> bisim2 pp visited H.
+Proof.
+intros. split. apply:bisim12. apply:bisim21.
+Qed.
+
+Lemma bisim_complete_aux : forall l0 l1 l_v, uniq_pair (l0,l1) ->  Extensional l0 l1 ->  bisim  (l0,l1) l_v.  
+Proof. 
+intros. funelim (bisim  (l0,l1) l_v).  rewrite -Heqcall. ssa.
+rewrite -Heqcall. ssa. 
+punfold H1.  inv H1. 
+rewrite foldInAllP. apply/allP=> x xIn. 
+apply:H. apply/inP. eauto.  simpl. 
+rewrite /uniq_pair /pd_l. ssa.
+punfold H1. inv H1. case: (H2 x)=>//. con. 
+done. rewrite  e1 in H. done.
+Qed.
+
+Lemma bisim_complete_aux2 : forall l0 l1 l_v (H : uniq_pair (l0,l1)),  Extensional l0 l1 ->  bisim2  (l0,l1) l_v H.  
+Proof.
+intros. apply/bisim_iff. apply:bisim_complete_aux. done. done.
+Qed.
+
+
+Definition undup2 pp := (undup pp.1,undup pp.2).
+Lemma pair_uniq_proof : forall pp, uniq_pair (undup2 pp). 
+Proof.
+intros. rewrite /uniq_pair. ssa.
+Qed.
+Definition bisim_wrap l l' := bisim2 (undup l,undup l') nil (pair_uniq_proof (l,l')).
+
+
+
+(*Check pd_plus.
+Lemma pd_plus : forall l a, pd a (\big[Plus/Empt]_(i <- l) i) = flatten (map (pd a) l).*)
+(*Theorem equiv_rInd : forall l l', Extensional l l' -> forall s, P s ( (\big[Plus/Empt]_(i <- l) i))  (\big[Plus/Empt]_(i <- l') i).
+Proof.
+move=> l0 l1 HC s. 
+elim: s l0 l1  HC.
+- move=> c0 c1. sunfold. case. move=> ce c3 HC HC'. 
+  rewrite -!Match_has_nu_iff. HC' //.
+- move=> a l IH c0 c1. sunfold. elim.
+  move=> c2 c3 /(_ a) [] // HC _. 
+  rewrite !deriveP2. rewrite /pd_sum. rewrite !pd_plus //.
+  apply/IH=>//. 
+Qed.*)
+
+(*Check Extensional_equiv.
+Lemma Extensional_equiv : forall l l', Extensional l l' <->  forall s, P s (\big[Plus/Empt]_(i <- l) i) (\big[Plus/Empt]_(i <- l') i). 
+Proof.
+intros. split. apply/equiv_rInd. move/equivP/Bisim_co_ind=>//.
+Qed.*)
+
+Lemma bisim_complete : forall l0 l1, Extensional l0 l1 ->  bisim_wrap l0 l1.
+Proof.
+intros. apply:bisim_complete_aux2. 
+apply/Extensional_equiv. 
+intro.
+apply -> P_undup. move: s.
+apply/Extensional_equiv=>//.
+Qed.
+
+
+Lemma bisim_sound_aux : forall e0 e1 l_v (R : @pder A -> @pder A -> Prop), (forall x0 x1, (x0,x1) \in l_v -> R x0 x1) ->   bisim (e0,e1) l_v -> upaco2 exten_gen R e0 e1. 
+Proof. 
+move => e0 e1 /= l_v R.  intros. funelim (bisim (e0,e1) l_v).
+right.  apply/H=>//=.
+left. pcofix CIH. pfold. rewrite -Heqcall in H1.
+destruct (andP H1).  ssa.
+rewrite foldInAllP in H3. con. 
+intros. eapply H. 3: {  apply (allP H3). done. } 3: { con. }  apply/inP. done. 
+intros. rewrite !inE in H1. de (orP H1). norm_eqs. inv H6. done. eauto.
+rewrite -Heqcall in H0. done.
+Qed.
+
+Lemma bisim_sound : forall e0 e1, bisim_wrap e0 e1 -> Extensional e0 e1.  
+Proof. move => e0 e1 H. 
+rewrite /bisim_wrap in H. apply bisim_iff in H. apply:Bisim_co_ind=>s. apply/P_undup.
+move: s. apply/Extensional_equiv.
+suff: upaco2 exten_gen bot2 (undup e0) (undup e1). case=>//=. 
+apply/bisim_sound_aux.  2:eauto. done.
+Qed.
+
+Definition decP (r0 r1 : @regex A) := bisim_wrap [::r0] [::r1].
+Lemma P_decidable : forall r0 r1, decP r0 r1 <-> forall s, P s r0 r1.
+Proof.
+intros. split. move/bisim_sound. move/Extensional_equiv.
+move=> H s. rewrite !big_cons !big_nil in H.
+intros. apply P_empt. done.
+intros. apply/bisim_complete. apply/Bisim_co_ind.
+intros. rewrite !big_cons !big_nil. apply P_empt. done.
+Qed.
+End Extensional.
