theories/regex.v
@@ -1,0 +1,388 @@
+From HB Require Import structures.
+From mathcomp Require Import all_ssreflect zify.
+From deriving Require Import deriving. 
+Require Import Containment.tactics.
+
+Set Implicit Arguments.
+Set Maximal Implicit Insertion.
+
+Let inE := tactics.inE.
+
+Section Regex.
+Variable (A : eqType).
+Inductive regex  : Type :=
+| Eps : regex
+| Empt : regex
+| Event : A -> regex
+| Plus : regex -> regex -> regex
+| Seq : regex -> regex -> regex
+| Star : regex -> regex.
+
+Definition regex_indDef := [indDef for regex_rect].
+Canonical regex_indType := IndType regex regex_indDef.
+
+Definition regex_hasDecEq := [derive hasDecEq for regex].
+HB.instance Definition _ := regex_hasDecEq.
+
+
+Notation "c0 _;_ c1"  := (Seq c0 c1)
+                         (at level 52, left associativity).
+
+Notation "c0 _+_ c1"  := (Plus c0 c1)
+                         (at level 53, left associativity).
+Definition trace := seq A.
+
+Fixpoint nu(c:regex ):bool :=
+match c with
+| Eps => true
+| Empt => false
+| Event e => false
+| Seq c0 c1 => nu c0 && nu c1
+| Plus c0 c1 => nu c0 || nu c1
+| Star c => true
+end.
+
+Inductive Match : trace -> regex -> Prop :=
+  | MEps : Match [::]  Eps
+  | MEvent x : Match [::x] (Event x)
+  | MSeq s1 c1 s2 c2 : Match s1 c1 ->  Match s2 c2 -> Match (s1 ++ s2) (c1 _;_ c2)
+  | MPlusL s1 c1 c2:  Match s1 c1 -> Match s1 (c1 _+_ c2)
+  | MPlusR c1 s2 c2:  Match s2 c2 ->  Match s2 (c1 _+_ c2)
+  | MStar0 c  : Match [::] (Star c)
+  | MStarSeq c s1 s2:  Match s1 c -> Match s2 (Star c) -> Match (s1 ++ s2) (Star c).
+Hint Constructors Match.
+
+Definition equiv (r0 r1: regex) := forall s, Match s r0 <-> Match s r1.
+
+
+Lemma MSeq2: forall s0 s1 c0 c1 s, Match s0 c0 -> Match s1 c1 -> s = s0 ++ s1  -> Match s (c0 _;_ c1).
+Proof.
+move => s0 s1 c0 c1 s HM0 HM1 Heq;subst. eauto.
+Qed.
+
+Lemma MStar2 : forall s0 s1 c s, Match s0 c -> Match s1 (Star c) -> s = s0 ++ s1  -> Match s (Star c).
+Proof.
+move => s0 s1 c s HM0 HM1 Heq;subst. eauto.
+Qed.
+
+
+
+Reserved Notation "e \ c" (at level 40, left associativity).
+Fixpoint derive (e:A) (c:regex) :regex :=
+match c with
+| Eps => Empt
+| Empt => Empt
+| Event e' => if e' == e then Eps else Empt
+| c0 _;_ c1 => if nu c0 then
+                 ((e \ c0) _;_ c1) _+_ (e \ c1)
+                 else (e \ c0) _;_ c1
+| c0 _+_ c1 => e \ c0 _+_ e \ c1
+| Star c => e \ c _;_ (Star c)
+end
+where "e \ c" := (derive e c).
+
+Reserved Notation "s \\ c" (at level 42, no associativity).
+Fixpoint trace_derive (s : trace) (c : regex)  : regex :=
+match s with
+| [::] => c
+| e::s' => s' \\ (e \ c)
+end
+where "s \\ c" := (trace_derive s c).
+
+Lemma derive_distr_plus : forall (s : trace)(c0 c1 : regex), s \\ (c0 _+_ c1) = s \\ c0 _+_ s \\ c1.
+Proof.
+induction s;intros;simpl;auto.
+Qed. 
+
+Hint Rewrite derive_distr_plus.
+
+
+Lemma nu_seq_trace_derive : forall (s : trace)(c0 c1 : regex), 
+nu c0 -> nu (s \\ c1) -> nu (s \\ (c0 _;_ c1)).
+Proof.
+induction s;intros;simpl in *. intuition. destruct (nu c0).
+rewrite derive_distr_plus. simpl. auto with bool. discriminate.
+Qed.
+
+Lemma matchb_seq : forall (s0 s1 : trace)(c0 c1 : regex), nu (s0\\c0) 
+                                                      -> nu (s1\\c1)-> nu ((s0++s1)\\(c0 _;_c1)).
+Proof.
+induction s0;intros;simpl in *.
+- rewrite nu_seq_trace_derive; auto. 
+- destruct (nu c0);first by rewrite derive_distr_plus /= IHs0//.
+  rewrite IHs0 //.
+Qed.
+
+Definition matchb s r := nu (trace_derive s r).
+
+Lemma Match_i_matchb : forall (c : regex)(s : trace), Match s c -> matchb s c.  
+Proof.
+move=> c s. rewrite /matchb. elim=>//=.
+- move => x. rewrite eqxx//.
+- move => s1 c1 s2 c2 HM0 HN0 HM1 HN1/=. by apply/matchb_seq=>//.
+- move=> s1 c1 c2 HM HN. rewrite derive_distr_plus /= HN//.
+- move=> c1 s2 c2 HM HN. rewrite derive_distr_plus /= HN orbC //.
+- move=> c0 []//= a l s2 HM HN HM' HN' /=. by apply/matchb_seq=>//.
+Qed.
+
+Lemma Match_nil_nu : forall (c : regex), nu c  -> Match [::] c.
+Proof.
+intros;induction c; simpl in H ; try discriminate; auto.
+- case: (orP H). move/IHc1;eauto. move/IHc2;eauto.
+- case: (andP H). move=>/IHc1 HH0 /IHc2 HH1. apply/MSeq2;eauto.
+Qed.
+
+Lemma Match_nil_seq: forall c0 c1, Match nil (Seq c0 c1) -> Match nil c0 /\ Match nil c1.
+Proof.
+move=> c0 c1 HM. inversion HM;subst. 
+destruct s1;ssa. destruct s2;ssa.
+Qed.
+
+Lemma nuP : forall c, nu c <-> Match [::] c.
+Proof.
+move=> c. con;first by apply/Match_nil_nu=>//.
+elim: c=>//=. move=> HM. inv HM. move=> s HM. inv HM.
+move=> r IH r0 HM HM2. apply/orP. inv HM2;eauto.
+move=> r IH r0 IH2 HM. apply/andP.
+move/Match_nil_seq: HM=>[]. eauto.
+Qed.
+
+Lemma Match_matchb : forall (c : regex)(e : A)(s : trace), Match s (e \ c)-> Match (e::s) c.
+Proof.
+induction c;intros; simpl in*; try solve [inversion H].
+- move: H. case Hcase:(_==_)=>// HM. rewrite (eqP Hcase).
+  inv HM;auto. inv HM.
+- inv H;eauto.
+- destruct (nu c1) eqn:Heqn.
+  * inv H.
+    ** inv H2. apply/MSeq2;eauto.
+    ** apply/MSeq2. apply/Match_nil_nu=>//. eauto. done.
+  * inv H. apply/MSeq2. eauto. eauto. done.
+- inversion H. apply/MStar2;eauto.
+Qed.
+
+Theorem  matchbP: forall (c : regex)(s : trace), Match s c <-> matchb s c. 
+Proof.
+move=> c s. rewrite /matchb.
+split;first by apply/Match_i_matchb=>//.
+elim: s c=>//;first by move=> c /Match_nil_nu=>//.
+move=> a l IH c /=. move/IH/Match_matchb=>//.
+Qed.
+
+Lemma deriveP : forall (c : regex)(e : A)(s : trace), Match (e::s) c <-> Match s (e \ c).
+Proof.
+by move=> c e s; rewrite !matchbP.
+Qed.
+
+Fixpoint pd a r := 
+match r with 
+| Eps => nil 
+| Empt => nil 
+| Event a' => if a == a' then Eps::nil else nil
+| Plus r0 r1 => (pd a r0) ++ (pd a r1)
+| Seq r0 r1 => if nu r0 then (map (fun x => Seq x r1) (pd a r0)) ++ (pd a r1) else (map (fun x => Seq x r1) (pd a r0))
+| Star r0 => map (fun x => x _;_ Star r0) (pd a r0)
+end.
+
+(*uniqueness of pd_l will become important later for decision procedure*)
+Definition pd_l a l := undup (flatten (map (pd a) l)).
+Definition pd_sum a r := \big[Plus/Empt]_(r <- (pd a r)) r.
+Definition pder := seq regex.
+
+Lemma Match_big_undup : forall l s, Match s (\big[Plus/Empt]_(i <- undup l) i)  <->  Match s ((\big[Plus/Empt]_(i <- l) i)).
+Proof.
+elim;ssa. case_if. rewrite !big_cons. split.
+move/H. eauto. intros. apply/H. inv H1;eauto. 
+clear H1 H.
+elim: l a H0 H4;ssa.  rewrite !inE in H0. de (orP H0). norm_eqs. rewrite big_cons. eauto. 
+rewrite big_cons. eauto. 
+rewrite !big_cons. split. intros. inv H1;eauto. constructor 5. apply/H. done.
+intros. inv H1;eauto. constructor 5. apply/H. done.
+Qed.
+
+Lemma Match_big_cat : forall l  l' s, Match s (\big[Plus/Empt]_(i <- l ++ l') i)  <->  Match s ((\big[Plus/Empt]_(i <- l) i) _+_  (\big[Plus/Empt]_(i <- l') i)).
+Proof.
+split.
+elim: l l' s. ssa. 
+move=> a l IH l' s.  rewrite /= !big_cons. intros. inv H. eauto.
+apply IH in H2. inv H2. eauto. eauto.
+elim: l l' s. ssa. rewrite big_nil in H.  inv H. inv H2.
+move=> a l IH l' s.  rewrite /= !big_cons. intros. inv H. inv H2. eauto. 
+constructor 5.
+apply:IH. eauto. eauto.
+Qed.
+
+Lemma Match_factor_r : forall l s r (F : regex -> regex), Match s (\big[Plus/Empt]_(i <- l) (F i _;_ r)) -> Match s (\big[Plus/Empt]_(i <- l) (F i) _;_ r). 
+Proof.
+elim;ssa. rewrite big_nil in H. inv H.
+move: H0. rewrite !big_cons. intros. inv H0. inv H3. eauto. 
+apply H in H3. inv H3. eauto.
+Qed.
+
+
+Lemma Match_factor_r2 : forall l s r (F : regex -> regex),  Match s (\big[Plus/Empt]_(i <- l) (F i) _;_ r) -> Match s (\big[Plus/Empt]_(i <- l) (F i _;_ r)). 
+Proof.
+elim;ssa. rewrite big_nil in H. inv H. inv H3.
+move: H0. rewrite !big_cons. intros. inv H0. inv H4. eauto. eauto.
+Qed.
+
+
+
+Lemma map_big_plus : forall l (f : regex -> regex), 
+\big[Plus/Empt]_(a <- map f l) a = \big[Plus/Empt]_(a <- l) (f a).
+Proof.
+elim;ssa.
+rewrite !big_nil. done.
+rewrite !big_cons. f_equal. done.
+Qed.
+
+Lemma has_nu_Match : forall l, Match [::] (\big[Plus/Empt]_(i <- l) i) ->  has nu l.
+Proof.
+elim;ssa. rewrite big_nil in H. inv H.
+rewrite !big_cons in H0. inv H0. 
+left. rewrite matchbP /matchb // in H3. eauto.
+Qed.
+
+Lemma Match_has_nu : forall l, has nu l ->  Match [::] (\big[Plus/Empt]_(i <- l) i).
+Proof.
+elim;ssa. de (orP H0). rewrite !big_cons /=. con.
+apply:Match_nil_nu. done.
+rewrite !big_cons. constructor 5. eauto.
+Qed.
+
+Lemma Match_has_nu_iff : forall l, has nu l <->  Match [::] (\big[Plus/Empt]_(i <- l) i).
+Proof.
+intros. split. apply/Match_has_nu. apply/has_nu_Match.
+Qed.
+
+Lemma der_eq : forall e r s, Match s (derive e r) <-> Match s (pd_sum e r).
+Proof.
+intros. rewrite /pd_sum. split.
+elim: r s e;ssa.  rewrite big_nil //. rewrite big_nil //.
+move: H. case_if. norm_eqs. rewrite eqxx. rewrite !big_cons big_nil. eauto.
+rewrite eq_sym H big_nil //=.
+inv H1. apply H in H4.
+move: H4. move: (pd e r0)=> l. 
+intros. apply/Match_big_cat. eauto.
+apply H0 in H4. apply/Match_big_cat. eauto.
+destruct (nu _) eqn:Heqn.  
+apply/Match_big_cat.  inv H1.  inv H4. 
+con.
+apply H in H6. 
+rewrite map_big_plus. apply Match_factor_r2. eauto. eauto. 
+inv H1.  apply H in H5.
+rewrite map_big_plus. apply Match_factor_r2. eauto.
+inv H0. rewrite map_big_plus. apply Match_factor_r2. eauto.
+
+rewrite /pd_sum.
+elim: r s e;ssa.  rewrite big_nil // in H. rewrite big_nil // in H.
+move: H. case_if. norm_eqs. rewrite eqxx. rewrite !big_cons big_nil. intros. inv H. inv H2. 
+rewrite eq_sym H big_nil //=. apply Match_big_cat in H1. inv H1. eauto. eauto.
+destruct (nu _) eqn:Heqn.  apply Match_big_cat in H1. inv H1. 
+rewrite map_big_plus in H4. apply Match_factor_r in H4. inv H4. eauto. eauto.
+rewrite map_big_plus in H1. apply Match_factor_r in H1. inv H1. eauto. 
+rewrite map_big_plus in H0. apply Match_factor_r in H0. inv H0. eauto.
+Qed.
+
+Lemma deriveP2
+     : forall (c : regex) (e : A) (s : trace),
+       Match (e :: s) c <-> Match s (pd_sum e  c).
+Proof. intros. 
+rewrite -der_eq. apply/deriveP.
+Qed.
+
+
+Lemma pd_plus : forall l e, undup (pd e (\big[Plus/Empt]_(i <- l) i)) = pd_l e l.
+Proof.
+rewrite /pd_l.
+elim;ssa.
+rewrite big_nil. done.
+rewrite big_cons /=. rewrite !undup_cat.  f_equal;try done. 
+apply/eq_in_filter. intro. ssa.   clear H0.
+move: x. clear H.  elim: l. ssa. rewrite big_nil. done. 
+intros. rewrite !big_cons /=.
+rewrite !mem_cat !negb_or. f_equal. eauto.
+Qed.
+
+Definition equiv_r (r0 r1 : regex) := forall s, Match s r0 <-> Match s r1.
+Definition contains_r (r0 r1 : regex) := forall s, Match s r0 -> Match s r1.
+
+
+End Regex.
+Arguments regex {A}.
+Arguments pder {A}.
+Arguments trace {A}.
+Arguments Eps {A}.
+Arguments Empt {A}.
+Arguments Event {A}.
+Arguments Plus {A}.
+Arguments Seq {A}.
+Arguments Star {A}.
+Notation "s \\ c" := (trace_derive s c)(at level 42, no associativity).
+Notation "s \ c" := (derive s c)(at level 42, no associativity).
+Notation "c0 _;_ c1"  := (Seq c0 c1)
+                         (at level 52, left associativity).
+
+Notation "c0 _+_ c1"  := (Plus c0 c1)
+                         (at level 53, left associativity).
+
+
+
+
+
+
+
+(*Lemma nu_seq_derive : forall (e : A)(c0 c1 : regex), 
+nu c0 -> nu (e \ c1) -> nu (e \ (c0 _;_ c1)).
+Proof.
+intros. simpl. destruct (nu c0). simpl. auto with bool. discriminate.
+Qed.
+*)
+(*Lemma nu_Empt : forall (s : trace)(c : regex), nu (s \\ (Empt _;_ c)) = false.
+Proof.
+induction s;intros. now simpl. simpl. auto.
+Qed.
+
+Hint Rewrite nu_Empt.
+
+Lemma nu_Eps : forall (s : trace)(c : regex), nu (s \\ (Eps _;_ c)) = nu (s \\ c).
+Proof.
+induction s;intros;simpl;auto. 
+by rewrite derive_distr_plus /= nu_Empt //=.
+Qed.*)
+
+(*Lemma deriveP3
+     : forall (c : regex) (e : A) (s : trace),
+       Match (e :: s) c <-> Match s (\big[Plus/Empt]_(i <- (pd e c)) i).
+Proof. intros. rewrite deriveP2 /pd_sum Match_big_undup //.
+Qed.*)
+
+
+
+
+(*Lemma seq_Eps : forall c, equiv (Eps _;_ c) c.
+Proof.
+move=> c s;split;intros. inversion H. inversion H3; subst. now simpl. by  apply/MSeq2;eauto.
+Qed. 
+
+Lemma seq_Empt : forall c, equiv (Empt _;_ c) Empt.
+Proof.
+move=> c s;split;intros. inversion H. inversion H3. inversion H.
+Qed.
+
+Hint Resolve seq_Eps seq_Empt.*)
+(*Fixpoint derive2 s l := 
+match s with 
+|nil => l 
+| a::s' =>derive2 s' (flatten (map (pd a) l))
+end.
+
+Lemma derive_nil : forall s, derive2 s nil = nil.
+Proof. elim;ssa.
+Qed.
+Lemma trace_derive_cat : forall s l0 l1, derive2 s (l0 ++ l1) = (derive2 s l0) ++ (derive2 s l1).
+Proof.
+elim;ssa=>//=.  
+elim: l0 l1 H;ssa. rewrite derive_nil /=. done.
+rewrite !H0. rewrite H. rewrite catA. done. done.
+Qed.*)
