theories/tactics.v
@@ -1,0 +1,76 @@
+From mathcomp Require Import all_ssreflect.
+Require Import Paco.paco.
+
+Ltac con := constructor. 
+Ltac econ := econstructor.
+
+Ltac case_if := match goal with 
+                | [ |- context[if ?X then _ else _ ]] => have : X by subst
+                | [ |- context[if ?X then _ else _ ]] => have : X = false by subst 
+
+                | [ |- context[if ?X then _ else _ ]] => let H := fresh in destruct X eqn:H
+
+                end; try (move=>->).
+
+Ltac rifliad := (repeat case_if); try done.
+
+Lemma neg_sym : forall (A : eqType) (a b : A), (a != b) = (b != a).
+Proof.
+intros. destruct (eqVneq a b).  done. done. 
+Qed.
+Locate split.
+Ltac split_ando :=
+  intros;
+   repeat
+    match goal with
+    | H:is_true (_ && _) |- _ => destruct (andP H); clear H
+    | H:_ && _ = true |- _ => destruct (andP H); clear H
+    | H:_ /\ _ |- _ => destruct H
+    | |- _ /\ _ => con
+    | |- is_true (_ && _) => apply /andP ; con
+    | |- is_true (_ || _) => apply /orP
+    | H : ex _ |- _ => destruct H
+    end; auto.
+
+
+Ltac split_and :=
+  intros;
+   repeat
+    match goal with
+    | H:is_true (_ && _) |- _ => destruct (andP H); clear H
+    | H:_ && _ = true |- _ => destruct (andP H); clear H
+    | H:_ /\ _ |- _ => destruct H
+    | |- _ /\ _ => con
+    | |- is_true (_ && _) => apply /andP ; con
+    | H : ex _ |- _ => destruct H
+    end; auto.
+
+
+Notation eq_iff := Bool.eq_iff_eq_true.
+Ltac ssa' := rewrite ?inE;simpl in *; split_and;try done.
+Ltac ssa := rewrite ?inE;simpl in *; split_ando;try done.
+
+Ltac ptac := 
+(match goal with 
+                   | [ H : is_true (_ \in (map _ _)) |- _ ] => move/mapP : H;case;intros;subst
+                   | [ H : is_true (_ \in (flatten _)) |- _ ] => move/flattenP : H;case;intros;subst
+                   | [ H : is_true (_ \in (filter _ _)) |- _ ] => move : H;rewrite mem_filter
+                   | [ H : is_true (_ \in (mem ((filter _ _)))) |- _ ] => move : H;rewrite mem_filter
+                  end);ssa.
+
+Ltac de i := destruct i;ssa.
+Ltac inv H := inversion H;subst;try done. 
+Ltac norm_eqs := repeat 
+(match goal with 
+                   | [ H : is_true (_ == _) |- _ ] => move : H => /eqP=>H
+                   | [ H : (_ == _) = true |- _ ] => move : H => /eqP=>H
+                   | [ H : (_ == _) = false |- _ ] => move : H => /negbT=>H
+
+                  end);subst;repeat (match goal with 
+                   | [ H : is_true (?a != ?a_) |- _ ] => rewrite eqxx in H;done 
+
+                  end).
+
+Let inE := (inE, eqxx,negb_or,negb_and).
+
+Ltac sunfold := let H := fresh "_Hunf" in move => H;punfold H;move : H.
